## Solve the model in terms of growth rates. How would you get a log linear approximate version of this model?

$$
y_{t}= A_{t}k_{t}^{\theta}h_{t}^{1-\theta} K_{t}^{1-\theta}
$$
Here, $k$ is capital per worker and $h$ is workers. That model is Romer's learning by doing model (1987). Instead, we will consider only the case $K_{t}=k_{t}$, so no externalities. That is like the AK model from Romer (1986) but in a simple Solow context, without endogenous saving. We therfore get: 
$$
y_{t}= A_{t}k_{t}h_{t}^{1-\theta}
$$
---

Usual equation of movement of capital

$$
(1+\lambda)k_{t+1}= (1-\delta )k_{t} + i_{t}
$$
If $i_{t}=s_{t}=s y_{t}$ and $A_{t}=A_{0}(1+\alpha)^{t}$, but $\alpha=0$. Then we get the Solow first difference equation:

$$
(1+\lambda)k_{t+1}= (1-\delta ) k_{t} + s  A_{0}k_{t}h_{t}^{1-\theta}
$$
Stationary state will be given by:
$$
k= \frac{1-\delta}{(1+\lambda)} k+ \frac{sA_{0}}{(1+\lambda)} kh^{1-\theta}
$$
There is only one solution where $k=0$. 

### Stochastic Technology Shocks
Using this stochastic process for technology:
$$
A_{t} = (1-\gamma) \bar{A} + \gamma A_{t-1} + \varepsilon _{t}
$$

where $\varepsilon_t$ is bounded both above and below and $|\gamma| < 1$.

The stochastic version of the Solow first difference equation becomes:
$$
(1+\lambda)k_{t+1}= (1-\delta ) k_{t} + s  A_{t}k_{t}h_{t}^{1-\theta}
$$

Substituting the technology process:
$$
(1+\lambda)k_{t+1}= (1-\delta ) k_{t} + s  [(1-\gamma) \bar{A} + \gamma A_{t-1} + \varepsilon _{t}]k_{t}h_{t}^{1-\theta}
$$

This can be written as:
$$
(1+\lambda)k_{t+1}= (1-\delta ) k_{t} + s(1-\gamma) \bar{A} k_{t}h_{t}^{1-\theta} + s\gamma A_{t-1} k_{t}h_{t}^{1-\theta} + s\varepsilon _{t} k_{t}h_{t}^{1-\theta}
$$
### Logs
Growth rate of the model:
$$
\gamma _{t} = \frac{k_{t+1}}{k_{t}}= \left( \frac{1-\delta }{(1+\lambda)}  + \frac{sA_{t}}{(1+\lambda)}h_{t}^{1-\theta} \right)
$$

Substituting the stochastic technology process:
$$
\gamma _{t} = \frac{1-\delta }{(1+\lambda)}  + \frac{s[(1-\gamma) \bar{A} + \gamma A_{t-1} + \varepsilon _{t}]}{(1+\lambda)}h_{t}^{1-\theta}
$$

Taking logs of both sides, we have a problem similar to the professor's notes. We need to manipulate the equation first. From the growth rate equation:
$$
\gamma _{t} - \frac{1-\delta }{1+\lambda} = \frac{s[(1-\gamma) \bar{A} + \gamma A_{t-1} + \varepsilon _{t}]}{(1+\lambda)}h_{t}^{1-\theta}
$$

Taking logs:
$$
\ln\left[\gamma _{t} - \frac{1-\delta }{1+\lambda}\right] = \ln\frac{s}{1+\lambda} + \ln[(1-\gamma) \bar{A} + \gamma A_{t-1} + \varepsilon _{t}] + (1-\theta)\ln h_{t}
$$

## Log-Linear Approximation

Following Professor McCandless' approach, we define $\tilde{k}_t = \ln(k_t) - \ln(\bar{k})$ where $\bar{k}$ is the stationary state value of capital, so $\tilde{k}_t = \ln(k_t/\bar{k})$.

Then $k_t = \bar{k} e^{\tilde{k}_t}$ and for the stochastic model:
$$
(1+\lambda) \bar{k} e^{\tilde{k}_{t+1}} = (1-\delta)\bar{k} e^{\tilde{k}_t} + s[(1-\gamma) \bar{A} + \gamma A_{t-1} + \varepsilon _{t}] \bar{k}^{\theta} \bar{h}^{1-\theta} e^{\theta\tilde{k}_t}
$$

Using the first-order Taylor approximation $e^{a\tilde{k}_t} \approx 1 + a\tilde{k}_t$ for small $\tilde{k}_t$:
$$
(1+\lambda) \bar{k}(1 + \tilde{k}_{t+1}) = (1-\delta)\bar{k}(1 + \tilde{k}_t) + s[(1-\gamma) \bar{A} + \gamma A_{t-1} + \varepsilon _{t}] \bar{k}^{\theta} \bar{h}^{1-\theta} (1 + \theta\tilde{k}_t)
$$

In stationary state: $(1+\lambda) \bar{k} = (1-\delta)\bar{k} + s\bar{A} \bar{k}^{\theta} \bar{h}^{1-\theta}$

The constant terms cancel out, leaving:
$$
(1+\lambda) \bar{k}\tilde{k}_{t+1} = (1-\delta)\bar{k}\tilde{k}_t + s(1-\gamma) \bar{A} \bar{k}^{\theta} \bar{h}^{1-\theta} + s\gamma A_{t-1} \bar{k}^{\theta} \bar{h}^{1-\theta} + s\varepsilon _{t} \bar{k}^{\theta} \bar{h}^{1-\theta} + s\bar{A} \bar{k}^{\theta} \bar{h}^{1-\theta} \theta\tilde{k}_t
$$

Since in steady state $s\bar{A} \bar{k}^{\theta} \bar{h}^{1-\theta} = (1+\lambda)\bar{k} - (1-\delta)\bar{k} = (\delta + \lambda)\bar{k}$, we get:
$$
\tilde{k}_{t+1} = \frac{(1-\delta) + (\delta + \lambda) \theta}{1+\lambda} \tilde{k}_t + \frac{s\gamma A_{t-1} \bar{k}^{\theta} \bar{h}^{1-\theta}}{(1+\lambda)\bar{k}} + \frac{(\delta + \lambda)}{1+\lambda} \varepsilon_t
$$

Defining $B = \frac{(1-\delta) + (\delta + \lambda) \theta}{1+\lambda}$ and $C = \frac{\delta + \lambda}{1+\lambda}$ and $D = \frac{s\gamma \bar{k}^{\theta-1} \bar{h}^{1-\theta}}{1+\lambda}$:

$$
\tilde{k}_{t+1} = B\tilde{k}_t + D A_{t-1} + C\varepsilon_t
$$

This gives us a log-linearized version of the stochastic Solow model with persistent technology shocks.